multi-step reduction

exercises/Smallstep.v
@@ -397,3 +397,317 @@ Qed.
 
 End Temp5.
 End Temp4.
+
+(* Multi-Step Reduction *)
+
+Inductive multi {X:Type} (R: relation X) : relation X :=
+  | multi_refl  : forall (x : X), multi R x x
+  | multi_step : forall (x y z : X),
+                    R x y ->
+                    multi R y z ->
+                    multi R x z.
+
+Tactic Notation "multi_cases" tactic(first) ident(c) :=
+  first;
+  [ Case_aux c "multi_refl" | Case_aux c "multi_step" ].
+
+Notation " t '==>*' t' " := (multi step t t') (at level 40).
+
+Theorem multi_R : forall (X:Type) (R:relation X) (x y : X),
+       R x y -> (multi R) x y.
+Proof.
+  intros X R x y H.
+  apply multi_step with y. apply H. apply multi_refl.   Qed.
+
+Theorem multi_trans :
+  forall (X:Type) (R: relation X) (x y z : X),
+      multi R x y  ->
+      multi R y z ->
+      multi R x z.
+Proof.
+  intros X R x y z G H.
+  multi_cases (induction G) Case.
+    Case "multi_refl". assumption.
+    Case "multi_step".
+      apply multi_step with y. assumption.
+      apply IHG. assumption.  Qed.
+
+(* Examples *)
+
+Lemma test_multistep_1:
+      P
+        (P (C 0) (C 3))
+        (P (C 2) (C 4))
+   ==>*
+      C ((0 + 3) + (2 + 4)).
+Proof.
+  apply multi_step with
+            (P
+                (C (0 + 3))
+                (P (C 2) (C 4))).
+  apply ST_Plus1. apply ST_PlusConstConst.
+  apply multi_step with
+            (P
+                (C (0 + 3))
+                (C (2 + 4))).
+  apply ST_Plus2. apply v_const.
+  apply ST_PlusConstConst.
+  apply multi_R.
+  apply ST_PlusConstConst. Qed.
+
+(** **** Exercise: 1 star, optional (test_multistep_2)  *)
+Lemma test_multistep_2:
+  C 3 ==>* C 3.
+Proof.
+  constructor. Qed.
+
+(** **** Exercise: 1 star, optional (test_multistep_3)  *)
+Lemma test_multistep_3:
+      P (C 0) (C 3)
+   ==>*
+      P (C 0) (C 3).
+Proof.
+  constructor. Qed.
+
+(** **** Exercise: 2 stars (test_multistep_4)  *)
+Lemma test_multistep_4:
+      P
+        (C 0)
+        (P
+          (C 2)
+          (P (C 0) (C 3)))
+  ==>*
+      P
+        (C 0)
+        (C (2 + (0 + 3))).
+Proof.
+  apply multi_step with (P (C 0) (P (C 2) (C (0 + 3)))).
+  repeat (apply ST_Plus2). constructor. constructor.
+  apply ST_PlusConstConst.
+  apply multi_step with (P (C 0) (C (2 + (0 + 3)))).
+  apply ST_Plus2. constructor. apply ST_PlusConstConst.
+  constructor.
+Qed.
+
+(* Normal Forms Again *)
+
+Definition step_normal_form := normal_form step.
+
+Definition normal_form_of (t t' : tm) :=
+  (t ==>* t' /\ step_normal_form t').
+
+(** **** Exercise: 3 stars, optional (normal_forms_unique)  *)
+Theorem normal_forms_unique:
+  deterministic normal_form_of.
+Proof.
+  unfold deterministic. unfold normal_form_of.  intros x y1 y2 P1 P2.
+  inversion P1 as [P11 P12]; clear P1. inversion P2 as [P21 P22]; clear P2.
+  generalize dependent y2.
+  multi_cases (induction P11) Case; intros.
+  Case "multi_refl".
+    multi_cases (inversion P21) SCase.
+    reflexivity.
+    apply ex_falso_quodlibet. apply P12. exists y. assumption.
+  Case "multi_step".
+    multi_cases (inversion P21) SCase; subst.
+    apply ex_falso_quodlibet. apply P22. exists y. apply H.
+    apply IHP11. apply P12.
+      assert (y0 = y). apply (step_deterministic x y0 y); assumption.
+      subst. assumption. assumption.
+Qed.
+
+Definition normalizing {X:Type} (R:relation X) :=
+  forall t, exists t',
+    (multi R) t t' /\ normal_form R t'.
+
+Lemma multistep_congr_1 : forall t1 t1' t2,
+     t1 ==>* t1' ->
+     P t1 t2 ==>* P t1' t2.
+Proof.
+  intros t1 t1' t2 H. multi_cases (induction H) Case.
+    Case "multi_refl". apply multi_refl.
+    Case "multi_step". apply multi_step with (P y t2).
+        apply ST_Plus1. apply H.
+        apply IHmulti.  Qed.
+
+(** **** Exercise: 2 stars (multistep_congr_2)  *)
+Lemma multistep_congr_2 : forall t1 t2 t2',
+     value t1 ->
+     t2 ==>* t2' ->
+     P t1 t2 ==>* P t1 t2'.
+Proof.
+  intros. multi_cases (induction H0) Case.
+  Case "multi_refl". constructor.
+  Case "multi_step". apply multi_step with (P t1 y).
+    apply ST_Plus2; assumption.
+    assumption.
+Qed.
+
+Theorem step_normalizing :
+  normalizing step.
+Proof.
+  unfold normalizing.
+  tm_cases (induction t) Case.
+    Case "C".
+      exists (C n).
+      split.
+      SCase "l". apply multi_refl.
+      SCase "r".
+        (* We can use [rewrite] with "iff" statements, not
+           just equalities: *)
+        rewrite nf_same_as_value. apply v_const.
+    Case "P".
+      inversion IHt1 as [t1' H1]; clear IHt1. inversion IHt2 as [t2' H2]; clear IHt2.
+      inversion H1 as [H11 H12]; clear H1. inversion H2 as [H21 H22]; clear H2.
+      rewrite nf_same_as_value in H12. rewrite nf_same_as_value in H22.
+      inversion H12 as [n1]. inversion H22 as [n2].
+      rewrite <- H in H11.
+      rewrite <- H0 in H21.
+      exists (C (n1 + n2)).
+      split.
+        SCase "l".
+          apply multi_trans with (P (C n1) t2).
+          apply multistep_congr_1. apply H11.
+          apply multi_trans with
+             (P (C n1) (C n2)).
+          apply multistep_congr_2. apply v_const. apply H21.
+          apply multi_R. apply ST_PlusConstConst.
+        SCase "r".
+          rewrite nf_same_as_value. apply v_const.  Qed.
+
+(* Equivalence of Big-Step and Small-Step Reduction *)
+
+(** **** Exercise: 3 stars (eval__multistep)  *)
+
+Theorem eval__multistep : forall t n,
+  t || n -> t ==>* C n.
+Proof.
+  intros.
+  eval_cases (induction H) Case.
+  Case "E_Const". constructor.
+  Case "E_Plus". apply multi_trans with (P (C n1) (C n2)).
+    apply multi_trans with (P (C n1) t2).
+    apply multistep_congr_1. assumption.
+    apply multistep_congr_2. apply nf_same_as_value. apply value_is_nf. constructor. assumption.
+    apply multi_step with (C (n1 + n2)).
+    apply ST_PlusConstConst. constructor.
+Qed.
+
+(** **** Exercise: 3 stars (step__eval)  *)
+Lemma step__eval : forall t t' n,
+     t ==> t' ->
+     t' || n ->
+     t || n.
+Proof.
+  intros t t' n Hs. generalize dependent n.
+  step_cases (induction Hs) Case; intros.
+  Case "ST_PlusConstConst".
+    inversion H. apply E_Plus; constructor.
+  Case "ST_Plus1".
+    inversion H. apply E_Plus. apply IHHs. assumption. assumption.
+  Case "ST_Plus2".
+    inversion H0. apply E_Plus. assumption. apply IHHs. assumption.
+Qed.
+
+
+(* Exercise: 3 stars (multistep__eval) *)
+
+Theorem multistep__eval : forall t t',
+  normal_form_of t t' -> exists n, t' = C n /\ t || n.
+Proof.
+  unfold normal_form_of. unfold step_normal_form.
+  intros. destruct H as [H1 H2]. apply nf_same_as_value in H2. inversion H2.
+  exists n. split. reflexivity.
+  multi_cases (induction H1) Case; subst.
+  Case "multi_refl". constructor.
+  Case "multi_step". apply step__eval with y. assumption.
+   apply IHmulti. constructor. reflexivity.
+Qed.
+
+(* Additional Exercises *)
+
+(* Exercise: 3 stars, optional (interp_tm) *)
+
+Theorem evalF_eval : forall t n,
+  evalF t = n <-> t || n.
+Proof.
+  split.
+  Case "->". generalize dependent n. tm_cases (induction t) SCase; intros.
+    SCase "C". simpl in H. subst. constructor.
+    SCase "P". simpl in H. subst. apply E_Plus.
+      apply IHt1. reflexivity.
+      apply IHt2. reflexivity.
+  Case "<-". intros.
+    eval_cases (induction H) SCase; subst; reflexivity.
+Qed.
+
+(* Exercise: 4 stars (combined_properties) *)
+
+
+Module Combined.
+
+Inductive tm : Type :=
+  | C : nat -> tm
+  | P : tm -> tm -> tm
+  | ttrue : tm
+  | tfalse : tm
+  | tif : tm -> tm -> tm -> tm.
+
+Tactic Notation "tm_cases" tactic(first) ident(c) :=
+  first;
+  [ Case_aux c "C" | Case_aux c "P"
+  | Case_aux c "ttrue" | Case_aux c "tfalse" | Case_aux c "tif" ].
+
+Inductive value : tm -> Prop :=
+  | v_const : forall n, value (C n)
+  | v_true : value ttrue
+  | v_false : value tfalse.
+
+Reserved Notation " t '==>' t' " (at level 40).
+
+Inductive step : tm -> tm -> Prop :=
+  | ST_PlusConstConst : forall n1 n2,
+      P (C n1) (C n2) ==> C (n1 + n2)
+  | ST_Plus1 : forall t1 t1' t2,
+      t1 ==> t1' ->
+      P t1 t2 ==> P t1' t2
+  | ST_Plus2 : forall v1 t2 t2',
+      value v1 ->
+      t2 ==> t2' ->
+      P v1 t2 ==> P v1 t2'
+  | ST_IfTrue : forall t1 t2,
+      tif ttrue t1 t2 ==> t1
+  | ST_IfFalse : forall t1 t2,
+      tif tfalse t1 t2 ==> t2
+  | ST_If : forall t1 t1' t2 t3,
+      t1 ==> t1' ->
+      tif t1 t2 t3 ==> tif t1' t2 t3
+
+  where " t '==>' t' " := (step t t').
+
+Tactic Notation "step_cases" tactic(first) ident(c) :=
+  first;
+  [ Case_aux c "ST_PlusConstConst"
+  | Case_aux c "ST_Plus1" | Case_aux c "ST_Plus2"
+  | Case_aux c "ST_IfTrue" | Case_aux c "ST_IfFalse" | Case_aux c "ST_If" ].
+
+Theorem step_deterministic:
+  deterministic step.
+Proof.
+  unfold deterministic. intros x y1 y2 H1 H2.
+  generalize dependent y2.
+  step_cases (induction H1) Case; intros; inversion H2; subst; try(solve by inversion 2); try(reflexivity).
+  Case "ST_Plus1". apply IHstep in H4. subst. reflexivity.
+  Case "ST_Plus2". apply IHstep in H6. subst. reflexivity.
+  Case "ST_If". apply IHstep in H5. subst. reflexivity.
+Qed.
+
+Theorem strong_progress : exists t,
+  ~ (value t \/ (exists t', t ==> t')).
+Proof.
+  unfold not.
+  exists (tif (C 0) (C 0) (C 0)).
+  intros. destruct H as [H1 | H2]; try (solve by inversion 3).
+Qed.
+
+End Combined.
